port descriptors, update makefile, setup nix rocq build

src/Descriptors.v
@@ -1,13 +1,16 @@
-From coqutil Require Import Word.Bitwidth.
+From Stdlib Require Import Strings.String.
+From coqutil Require Import Word.Interface.
+From Flocq Require Import IEEE754.Binary.
+From Perennial Require Import Helpers.Word.Integers.
 From stdpp Require Import gmap.
 From stdpp Require Import mapset.
 
 Module Descriptors.
 
-  Inductive decorator :=
-  | IMPLICIT
-  | OPTIONAL
-  | REPEATED.
+  Inductive deco_desc :=
+  | D_IMPLICIT
+  | D_OPTIONAL
+  | D_REPEATED.
   
   Definition reserved_id := nat.
   (* Which one of these should the later definitions use? While I think that the prop is largely
@@ -15,19 +18,31 @@ Module Descriptors.
   Definition reserved_set := (mapset (gmap reserved_id)).
   Definition reserved_set_prop := FinSet reserved_id reserved_set.
 
-  Inductive field_desc : Type :=
-  | F_DOUBLE : decorator -> field_desc
-  | F_FLOAT : decorator -> field_desc
-  | F_INT : Bitwidth -> decorator -> field_desc
-  | F_UINT : decorator -> field_desc
-  | F_SINT : decorator -> field_desc
-  | F_FIXED : decorator -> field_desc
-  | F_SFIXED : decorator -> field_desc
-  | F_BOOL : decorator -> field_desc
-  | F_STRING : decorator -> field_desc
-  | F_BYTES : decorator -> field_desc
-  | F_MSG : msg_desc -> decorator -> field_desc
-  | F_ENUM : decorator -> field_desc
+  Definition width_prop (n : nat) : Prop := n = 32%nat \/ n = 64%nat.
+  Definition width := {n : nat | width_prop n }.
+
+  Lemma width_32_prop : width_prop 32.
+  Proof. unfold width_prop. left. reflexivity. Qed.
+
+  Lemma width_64_prop : width_prop 64.
+  Proof. unfold width_prop. right. reflexivity. Qed.
+
+  Definition width32 : width := exist width_prop 32 width_32_prop.
+  Definition width64 : width := exist width_prop 64 width_64_prop.
+
+  Inductive val_desc : Type :=
+  | D_DOUBLE :            deco_desc -> val_desc
+  | D_FLOAT  :            deco_desc -> val_desc
+  | D_INT    :    width -> deco_desc -> val_desc
+  | D_UINT   :    width -> deco_desc -> val_desc
+  | D_SINT   :    width -> deco_desc -> val_desc
+  | D_FIXED  :    width -> deco_desc -> val_desc
+  | D_SFIXED :    width -> deco_desc -> val_desc
+  | D_BOOL   :            deco_desc -> val_desc
+  | D_STRING :            deco_desc -> val_desc
+  | D_BYTES  :            deco_desc -> val_desc
+  | D_MSG    : msg_desc -> deco_desc -> val_desc
+  | D_ENUM   :            deco_desc -> val_desc
                       
   (*
     Looks like I can't define a mfield_desc as a record, like in F*, since I'm getting this error:
@@ -42,6 +57,111 @@ Module Descriptors.
     Although, without providing an example, it does claim that mutually inductive record
     definitions are allow if "as long as all of the types in the block are records."
    *)
-    with msg_desc : Type := D_MSG : reserved_set -> list field_desc -> msg_desc.
+    with field_desc := D_FIELD : string -> nat -> val_desc -> field_desc
+    with msg_desc := D_MESSAGE : reserved_set -> list field_desc -> msg_desc.
 
+  Definition field_desc_get_name (f:field_desc) : string :=
+    match f with
+    | D_FIELD name _ _ => name
+    end.
+  
+  Definition field_desc_get_id (f:field_desc) : nat :=
+    match f with
+    | D_FIELD _ id _ => id
+    end.
+
+  Definition field_desc_get_val (f:field_desc) : val_desc :=
+    match f with
+    | D_FIELD _ _ val => val
+    end.
+
+  Definition msg_desc_get_reserved (m:msg_desc) : reserved_set :=
+    match m with
+    | D_MESSAGE rset _ => rset
+    end.
+
+  Definition msg_desc_get_fields (m:msg_desc) : list field_desc :=
+    match m with
+    | D_MESSAGE _ fields => fields
+    end.
+
+  Inductive deco_val {v : Type} : Type :=
+    | V_IMPLICIT : v -> deco_val
+    | V_OPTIONAL : option v -> deco_val
+    | V_REPEATED : list v -> deco_val.
+
+  Definition f32 := binary_float 24 128.
+  Definition f32_zero := B754_zero 24 128 false.
+  Definition f64 := binary_float 53 1024.
+  Definition f64_zero := B754_zero 53 1024 false.
+  
+  Inductive val_val :=
+  | V_DOUBLE : @deco_val f64 -> val_val
+  | V_FLOAT  : @deco_val f32 -> val_val
+  | V_INT    : @deco_val Z -> val_val
+  | V_BOOL   : @deco_val bool -> val_val
+  | V_STRING : @deco_val string -> val_val
+  | V_BYTES  : @deco_val (list u8) -> val_val
+  | V_MSG    : @deco_val msg_val -> val_val
+  | V_ENUM   : @deco_val unit -> val_val
+
+  with field_val := V_FIELD : string -> val_val -> field_val
+  with msg_val := V_MESSAGE : list field_val -> msg_val.
+
+  Definition empty_message : msg_val := V_MESSAGE nil.
+  
+  (* MESSAGE INITIALIZATION *)
+
+  Definition init_deco {A : Type} (deco : deco_desc) (def : A) :=
+    match deco with
+    | D_IMPLICIT => V_IMPLICIT def
+    | D_OPTIONAL => V_OPTIONAL None
+    | D_REPEATED => V_REPEATED nil
+    end.
+
+  (* I originally had each function accessible and mutually recursive via the 'with' keyword,
+     but coq kept complaining about ill-formed recursive definitions at the init_field call
+     in init_fields. That would be sound in the sense that any potential calls back to init_msg
+     are operating over a different msg_desc, Rocq didn't seem to think so. Per this stackexchange
+     post, this issue can be fixed by moving the fixpoints inside one another, although I'm not sure
+     why this helps.
+
+     https://cs.stackexchange.com/a/120
+   *)
+  Fixpoint init_msg (m:msg_desc) : msg_val := 
+  let init_field := (fix init_field (f:field_desc) : field_val :=
+    V_FIELD (field_desc_get_name f)
+      (match (field_desc_get_val f) with
+       | D_DOUBLE dd => V_DOUBLE (init_deco dd f64_zero)
+       | D_FLOAT dd => V_FLOAT (init_deco dd f32_zero)
+       | D_INT _ dd
+       | D_UINT _ dd
+       | D_SINT _ dd
+       | D_FIXED _ dd
+       | D_SFIXED _ dd => V_INT (init_deco dd 0%Z)
+       | D_BOOL dd => V_BOOL (init_deco dd false)
+       | D_STRING dd => V_STRING (init_deco dd EmptyString)
+       | D_BYTES dd => V_BYTES (init_deco dd nil)
+       | D_MSG m dd => V_MSG (init_deco dd (init_msg m))
+       | D_ENUM dd => V_ENUM (init_deco dd ())
+       end)) in
+  let init_fields := (fix init_fields (fs:list field_desc) : list field_val :=
+    match fs with
+    | nil => nil
+    | hd :: tl => init_field hd :: init_fields tl
+    end) in
+  V_MESSAGE (init_fields $ msg_desc_get_fields m).
+
+(* TODO / FIXME:
+
+   What has been lost porting from F*?
+
+   There is no longer type-level enforcements that the list of field descriptors
+   have unique field id numbers and names. In F* that was defined via a refinement on
+   the list of field descriptors. This file uses Rocq's refinement types, but having to
+   manually prove that each element is in the refinement is frankly annoying, so while
+   it works for something as simple as the bit width, I going to try to avoid it in
+   the rest of the port. This property on the descriptors will need to be restored via
+   a predicate over the descriptor and proven or assumed in all the proofs.
+ *)
 End Descriptors.
