nix/pollux-rocq/default.nix
@@ -1,0 +1,34 @@
+{
+  stdenv,
+  rocq-core,
+  rocqPackages,
+  perennial,
+  flocq,
+  ...
+}:
+stdenv.mkDerivation {
+  pname = "pollux-rocq";
+  version = "unstable";
+
+  src = ../../.;
+
+  nativeBuildInputs = [
+    rocq-core
+  ];
+  buildInputs = [
+    perennial
+    flocq
+    rocqPackages.stdlib
+  ];
+
+  enableParallelBuilding = true;
+
+  buildPhase = ''
+    make -j$NIX_BUILD_CORES
+  '';
+
+  installPhase = ''
+    mkdir -p $out/lib/coq/${rocq-core.rocq-version}/user-contrib
+    cp -r src $out/lib/coq/${rocq-core.rocq-version}/user-contrib/Pollux
+  '';
+}
